vacaciones

Especificaciones/Auxiliar/Graph.dfy
@@ -32,6 +32,25 @@ requires isValidGraph(B)
     A.0 <= B.0 && A.1 <= B.1
 }
 
+lemma corollaryToValidity(graph: Graph, S: set<Node>)
+requires isValidGraph(graph)
+requires graph.0 * S == {}
+ensures forall n: Node, e: Edge | n in S && e in graph.1 :: n !in e
+{ }
+
+lemma existenceImpliesNonEmpty<T>(A: set<T>, B: set<set<T>>)
+requires forall x: T | x in A :: (exists y: set<T> :: y in B && x in y)
+ensures forall x: T | x in A :: (set y: set<T> | y in B && x in y :: y) != {}
+{ 
+    if exists x: T :: x in A && (set y: set<T> | y in B && x in y :: y) == {} {
+        var x: T :| x in A && (set y: set<T> | y in B && x in y :: y) == {}; 
+        var setX: set<set<T>> := (set y: set<T> | y in B && x in y :: y);
+        assert forall y: set<T> | y in B && x in y :: y in setX;
+        assert setX == {};
+        assert forall y: set<T> | y in B :: x !in y;
+    }
+}
+
 lemma intersect(s: set<Node>, graph:Graph, e: Edge, u: Node, v: Node)
 requires isValidGraph(graph)
 requires e in graph.1
@@ -84,52 +103,168 @@ ensures e in edgesToChange
     pickedEdge
 }
 
+function newSplitEdgesRec(graph: Graph, newNodes: set<Node>, newNodesRemaining: set<Node>, edgesToChange: set<Edge>, removedNode: Node, setAnalyzedNodes: set<Node>, setCreatedEdges: set<Edge>): (r: set<Edge>)
+requires isValidGraph(graph)
+requires removedNode in graph.0
+requires edgesToChange <= graph.1
+requires forall edge: Edge | edge in edgesToChange :: removedNode in edge && |edge| == 2
+requires removedNode !in newNodes
+requires |edgesToChange| == |newNodesRemaining|
+requires |setAnalyzedNodes| == |setCreatedEdges|
+requires newNodes * graph.0 == {}
+requires newNodesRemaining <= newNodes
+requires newNodesRemaining * graph.0 == {}
+requires setAnalyzedNodes * newNodesRemaining == {}
+requires setAnalyzedNodes + newNodesRemaining == newNodes
+requires forall e: Edge | e in edgesToChange :: (exists n: Node :: n in e && n in neighborsOf(graph, removedNode))
+requires forall n: Node | n in setAnalyzedNodes :: ((exists e: Edge :: e in setCreatedEdges && n in e))  
+requires forall n: Node, e: Edge | n !in setAnalyzedNodes && n !in (graph.0 - {removedNode}) && e in setCreatedEdges :: n !in e
+requires forall n: Node | n in setAnalyzedNodes :: ((exists e: Edge :: e in setCreatedEdges && n in e)) 
+decreases edgesToChange
+ensures forall e: Edge | e in r :: |e| == 2 
+ensures forall n: Node, e: Edge | n !in newNodesRemaining && n !in (graph.0 - {removedNode}) && e in r :: n !in e 
+ensures forall e: Edge | e in r :: (exists node1: Node, node2: Node :: node1 in newNodes && node2 in (graph.0 - {removedNode}) && e == {node1, node2}) 
+ensures forall n: Node | n in newNodes :: ((exists e: Edge :: e in (r + setCreatedEdges) && n in e))
+//ensures forall e: Edge | e in r :: (exists n: Node :: n in e && n in neighborsOf(graph, removedNode))
+ensures forall n: Node | n in newNodesRemaining :: (|(set e: Edge | e in r && n in e :: e)| == 1)
+{
+    if edgesToChange == {} then 
+        assert setAnalyzedNodes == newNodes;
+        assert forall n: Node | n in setAnalyzedNodes :: (exists e: Edge :: e in setCreatedEdges && n in e);
+        {}
+    else
+        //Functionality
+        var node: Node := pickMax(newNodesRemaining);
+        var changedEdge: Edge := pickEdgeFromNode(newNodesRemaining, edgesToChange, removedNode);
+        var edge' := changedEdge - {removedNode};
+        var edge'' := edge' + {node};
+        assert node !in setAnalyzedNodes;
+        assert edge'' !in setCreatedEdges;
+        var remainingEdges: set<Edge> := newSplitEdgesRec(graph, newNodes, newNodesRemaining - {node}, edgesToChange - {changedEdge}, removedNode, setAnalyzedNodes + {node}, setCreatedEdges + {edge''});
+        var rv: set<Edge> := {edge''} + remainingEdges;
+
+        //No particular proof needed
+        assert forall e: Edge | e in rv :: |e| == 2 ;
+        assert forall n: Node, e: Edge | n !in newNodesRemaining && n !in (graph.0 - {removedNode}) && e in rv :: n !in e; 
+        assert forall n: Node | n in newNodes :: ((exists e: Edge :: e in (rv + setCreatedEdges) && n in e));
+
+        //Proof for forall e: Edge | e in r :: (exists node1: Node, node2: Node :: node1 in newNodes && node2 in (graph.0 - {removedNode}) && e == {node1, node2})  
+        assert exists n: Node :: n in (graph.0 - {removedNode}) && n in edge';
+        ghost var nodeFromGraph: Node :| nodeFromGraph in (graph.0 - {removedNode}) && nodeFromGraph in edge';
+        assert edge'' == {node, nodeFromGraph};
+        assert forall e: Edge | e in rv :: (exists node1: Node, node2: Node :: node1 in newNodes && node2 in (graph.0 - {removedNode}) && e == {node1, node2});
+
+        //Proof for forall n: Node | n in newNodes :: (|(set e: Edge | e in r && n in e :: e)| == 1)
+        
+        ghost var setEdge: set<Edge> := (set e: Edge | e in {edge''} && node in e :: e);
+        assert setEdge == {edge''};
+        ghost var setEdgeEmpty := (set e: Edge | e in remainingEdges && node in e :: e);
+        assert setEdgeEmpty == {};
+        assert (set e: Edge | e in rv && node in e :: e) == setEdge + setEdgeEmpty;
+        cardinalitySum(setEdge, setEdgeEmpty);
+        assert |setEdge + setEdgeEmpty| == 1;
+        assert rv == rv;
+        assert rv == (setEdge + remainingEdges);
+        assert forall e: Edge :: e in rv <==> e in rv;
+        equalityBelonging(rv, (setEdge + remainingEdges));
+        assert forall e: Edge :: e in rv <==> e in (setEdge + remainingEdges);
+        //DUDA
+        assert forall e: Edge :: e in (set e: Edge | e in rv && node in e :: e) <==> (e in (setEdge + remainingEdges) && node in e);
+        assume false;
+        assert (set e: Edge | e in rv && node in e :: e) == setEdge + setEdgeEmpty;
+        cardinalitySum(setEdge, setEdgeEmpty);
+        assert |setEdge + setEdgeEmpty| == 1;
+        equialityImpliesSameCardinal((set e: Edge | e in rv && node in e :: e), (setEdge + setEdgeEmpty));
+        assert |(set e: Edge | e in rv && node in e :: e)| == |setEdge + setEdgeEmpty|;
+        assert forall n: Node | n in newNodesRemaining && n == node :: (|(set e: Edge | e in rv && n in e :: e)| == 1);
+        assert forall n: Node, e: Edge | n in newNodesRemaining && n != node && e in setCreatedEdges :: n !in e;
+        assert forall n: Node | n in newNodes :: ((exists e: Edge :: e in (rv + setCreatedEdges) && n in e));
+        assert forall n: Node, e: Edge | n in newNodesRemaining && n != node && e in setCreatedEdges :: n !in e;
+        
+        /*
+        assert forall n: Node | n in newNodesRemaining :: (|(set e: Edge | e in rv && n in e :: e)| >= 1) by {
+            //assert forall n: Node | n in newNodes :: ((exists e: Edge :: e in (rv + setCreatedEdges) && n in e));
+            //assert forall n: Node | n in newNodesRemaining :: ((exists e: Edge :: e in (rv + setCreatedEdges) && n in e));
+            //assert forall n: Node | n in newNodesRemaining :: n !in setAnalyzedNodes && n !in graph.0 - {removedNode};
+            //assert forall n: Node, e: Edge | n !in setAnalyzedNodes && n !in (graph.0 - {removedNode}) && e in setCreatedEdges :: n !in e;
+            //assert forall n: Node, e: Edge | n in newNodesRemaining && e in setCreatedEdges :: n !in e;
+            //assert forall n: Node | n in newNodesRemaining :: (exists e: Edge :: e in rv && n in e);
+            //existenceImpliesNonEmpty(newNodesRemaining, rv);
+            //assert forall n: Node | n in newNodesRemaining :: (set e: Edge | e in rv && n in e :: e) != {};
+        }
+        */
+        rv
+        
+}
 
 function newSplitEdges(graph: Graph, newNodes: set<Node>, edgesToChange: set<Edge>, removedNode: Node): (r: set<Edge>)
 requires isValidGraph(graph)
 requires removedNode in graph.0
 requires edgesToChange <= graph.1
 requires forall edge: Edge | edge in edgesToChange :: removedNode in edge && |edge| == 2
+requires removedNode !in newNodes
 requires |edgesToChange| == |newNodes|
 requires newNodes * graph.0 == {}
+requires forall e: Edge | e in edgesToChange :: (exists n: Node :: n in e && n in neighborsOf(graph, removedNode))
 decreases edgesToChange
-ensures forall e: Edge | e in r :: |e| == 2 && (exists node1: Node, node2: Node :: node1 in newNodes && node2 in graph.0 && e == {node1, node2})  
+ensures forall e: Edge | e in r :: |e| == 2 
+ensures forall n: Node, e: Edge | n !in newNodes && n !in (graph.0 - {removedNode}) && e in r :: n !in e 
+ensures forall e: Edge | e in r :: (exists node1: Node, node2: Node :: node1 in newNodes && node2 in (graph.0 - {removedNode}) && e == {node1, node2}) 
+//ensures forall n: Node | n in newNodes :: ((exists e: Edge :: e in r && n in e))
+ensures forall e: Edge | e in r :: (exists n: Node :: n in e && n in neighborsOf(graph, removedNode))
+ensures forall n: Node | n in newNodes :: (|(set e: Edge | e in r && n in e :: e)| == 1)
 {
-    if edgesToChange == {} then {}
-    else 
-        
-        var node: Node := pickMax(newNodes);
-        assert node !in graph.0 by{
-            assert node in newNodes;
-            assert newNodes * graph.0 == {};
-            if node in graph.0 {
-                assert node in graph.0 && node in newNodes;
-                assert node in newNodes * graph.0;
-                assert newNodes * graph.0 == {};
-                assert false;
-            }
-            assert node !in graph.0;
-        }
-        assert |edgesToChange| == |newNodes|;
-        var changedEdge: Edge := pickEdgeFromNode(newNodes, edgesToChange, removedNode);
-        assert |edgesToChange| == |newNodes|;
-        assert changedEdge in edgesToChange;
-        ghost var edge' := changedEdge - {removedNode};
-        assert |edge'| == 1; 
-        ghost var edge'' := edge' + {node};
-        assert !(node in edge');
-        assert |edge''| == 2;
-        {changedEdge - {removedNode} + {node}} + newSplitEdges(graph, newNodes - {node}, edgesToChange - {changedEdge}, removedNode)
+    var setAnalyzedNodes: set<Node> := {};    
+    newSplitEdgesRec(graph, newNodes, newNodes, edgesToChange, removedNode, {}, {})  
+}
+
+lemma incidentEdgesContainsNeighbors(g: Graph, n: Node, I: set<Edge>)
+    requires isValidGraph(g)
+    requires n in g.0
+    requires incidentEdges(g, n) == I
+    ensures forall e: Edge | e in I :: (exists node: Node :: node in e && node in neighborsOf(g, n))
+{
+    //exists e: Edge :: e in I && (forall node: Node | node in neighborsOf(g, n) :: node !in e)
+    if !forall e: Edge | e in I :: (exists node: Node :: node in e && node in neighborsOf(g, n)) {
+        //DUDA
+        assert exists e: Edge :: e in I && (forall node: Node | node in neighborsOf(g, n) :: node !in e);
+        var e: Edge :|  e in I;// :| e in I && (forall node: Node | node in neighborsOf(g, n) :: node !in e);
+        assume{:axiom} e in I && (forall node: Node | node in neighborsOf(g, n) :: node !in e);
+        var S: set<Node> := neighborsOf(g, n);
+        neighborsAreConnected(g, n, S);
+        assert forall m: Node | n in S :: {m, n} in incidentEdges(g, n); 
+        assert exists m: Node :: m in g.0 && m in e && n != m;
+        var m: Node :| m in g.0 && e == {n,m};
+    }
 }
 
 function incidentEdges(graph: Graph, node: Node) : (S: set<Edge>)
+    requires isValidGraph(graph)
+    ensures forall e: Edge | e in S :: |e| == 2
+    ensures forall e: Edge | e in S :: exists n: Node :: n in graph.0 && n in e && n != node
+    ensures forall e: Edge | e in graph.1 :: e in S <==> node in e
+    ensures forall e: Edge | e in graph.1 && node in e :: e in S
 {
     (set edge: Edge | edge in graph.1 && node in edge :: edge)
 }
 
-function neighborsOf(graph: Graph, v: Node) : (S: set<Node>)
+lemma neighborsAreConnected(g: Graph, n: Node, S: set<Node>)
+    requires isValidGraph(g)
+    requires n in g.0
+    requires S == neighborsOf(g, n)
+    ensures forall m: Node | n in S :: {m, n} in g.1 
 {
-    (set node: Node | node in graph.0  && {node, v} in graph.1 :: node)
+    if exists m: Node :: m in S && {m, n} !in g.1 {
+        assert forall node: Node | node in S :: {n, node} in g.1;
+    }
+}
+
+function neighborsOf(graph: Graph, v: Node) : (S: set<Node>)
+    requires isValidGraph(graph)
+    requires v in graph.0
+    ensures forall n: Node | n in S :: n in graph.0 && n != v
+{
+    (set node: Node | node in graph.0  && {v, node} in graph.1 :: node)
 }
 
 function removeVertex(graph: Graph, v: Node): (graph': Graph) 
@@ -151,23 +286,130 @@ requires isValidGraph(graph)
     else {}
 }
 
+lemma removeVertexValid(g: Graph, v: Node)
+    requires isValidGraph(g)
+    requires v in g.0
+    ensures isValidGraph((g.0 - {v}, g.1 - incidentEdges(g, v)))
+{
+    assert forall e | e in g.1 :: (|e| == 2 && exists u,v :: u in g.0 && v in g.0 && u != v && e == {u,v}); 
+}
+
+lemma notAVertexImpliesNotInAnEdge(graph: Graph, n: Node)
+requires isValidGraph(graph)
+requires n !in graph.0
+ensures forall e: Edge | e in graph.1 :: n !in e
+{ }
+
+lemma notAVertexImpliesNotInAnEdgeSet(graph: Graph, S: set<Node>)
+requires isValidGraph(graph)
+requires forall n: Node | n in S :: n !in graph.0
+ensures forall e: Edge, n: Node | e in graph.1 && n in S :: n !in e
+{ }
+
 //Given a graph and a vertex
 function splitVertex(graph: Graph, v: Node): (r: Graph)
 requires isValidGraph(graph) 
 ensures isValidGraph(r)
+//ensures forall n: Node | n in (r.0 - graph.0) :: |(set e: Edge | e in (r.1) && n in e :: e)| == 1
 {
+    
     //If it belongs to the graph
     if v in graph.0 then 
+        //The vertex is "split" such that all those edges still exist but connect to different new nodes
+        var edgesToChange: set<Edge> := incidentEdges(graph, v);
+        var newNodes: set<Node> := addMultipleGreater(graph.0, |edgesToChange|); 
+        assert(|newNodes| == |edgesToChange|);
+        incidentEdgesContainsNeighbors(graph, v, edgesToChange);
+        var setNewEdges: set<Edge> := newSplitEdges(graph, newNodes, edgesToChange, v);
+        var g := ((graph.0 - {v} + newNodes), (graph.1 - edgesToChange + setNewEdges));
+
+        //Proof for isValidGraph(r)
+        
+        assert forall e | e in setNewEdges :: |e| == 2;
+        assert forall e | e in setNewEdges :: (exists a, b :: a in newNodes && b in (graph.0 - {v}) && a != b && e == {a, b});
+        assert newNodes <= g.0;
+        removeVertexValid(graph, v);
+        assert isValidGraph((graph.0 - {v}, graph.1 - incidentEdges(graph, v)));
+        assert g.1 == graph.1 - incidentEdges(graph, v) + setNewEdges;
+        assert forall e: Edge | e in graph.1 :: (|e| == 2 && exists u,v :: u in graph.0 && v in graph.0 && u != v && e == {u,v});
+        //DUDA
+        //ensures forall e: Edge | e in graph.1 && node in e :: e in S
+        assert forall e: Edge | e in graph.1 && v in e :: e in incidentEdges(graph, v);
+        assume{:axiom} false;
+        assert forall e: Edge | e in graph.1 && v !in e :: e in (graph.1 - incidentEdges(graph, v));
+        setBelongingToDifferenceForAll(graph.0, v);
+        assert forall e | e in (graph.1 - incidentEdges(graph, v)) :: (|e| == 2 && exists node1, node2 :: node1 in (graph.0) && node2 in (graph.0) && node1 != node2 && node1 != v && node2 != v && node1 in (graph.0 - {v}) && node2 in (graph.0 - {v}) && e == {node1,node2});
+        assert forall e | e in (graph.1 - incidentEdges(graph, v)) :: (|e| == 2 && exists node1, node2 :: node1 in (graph.0 - {v}) && node2 in (graph.0 - {v}) && node1 != node2 && e == {node1,node2});
+        assert (graph.0 - {v}) <= g.0;
+        assert newNodes <= g.0;
+        assert forall e: Edge | e in setNewEdges :: (exists node1: Node, node2: Node :: node1 in newNodes && node2 in (graph.0 - {v}) && e == {node1, node2}); 
+        assert g.1 == graph.1 - incidentEdges(graph, v) + setNewEdges;
+        assert forall e | e in g.1 :: (|e| == 2 && exists u,v :: u in g.0 && v in g.0 && u != v && e == {u,v}); 
+        assert isValidGraph(g);
+        
+        //Proof for forall n: Node | n in (r.0 - graph.0) :: |(set e: Edge | e in (r.1) && n in e :: e)| == 1
+        
+        assert isValidGraph(graph);
+        assert forall A: Graph, B: set<Node>, C: set<Edge> | A == (B, C) :: A.0 == B && A.1 == C;
+        assert g.0 == graph.0 - {v} + newNodes;
+        assert graph.0 * newNodes == {};
+        setBelongingImplication(graph.0, v);
+        setDifference(g.0, graph.0, newNodes, {v});
+        assert (g.0 - graph.0) == newNodes;
+        corollaryToValidity(graph, newNodes);
+        assert forall n: Node, e: Edge | n in newNodes && e in graph.1 ::  n !in e;
+        assert forall n: Node | n in newNodes :: (|(set e: Edge | e in setNewEdges && n in e :: e)| == 1);
+        //assert forall n: Node | n in newNodes :: n !in graph.0;
+        //assert isValidGraph(graph);
+        //notAVertexImpliesNotInAnEdgeSet(graph, newNodes);
+        //assert forall e: Edge, n: Node | e in graph.1 && n in newNodes :: n !in e;
+
+        g
+        
+    //If the vertex does not belong to the graph, it remains unchanged
+    else graph
+}
+/*
+//Given a graph and a vertex
+function splitVertex(graph: Graph, v: Node): (r: Graph)
+requires isValidGraph(graph) 
+ensures isValidGraph(r)
+//ensures forall n: Node | n in (r.0 - graph.0) :: |(set e: Edge | e in (r.1) && n in e :: e)| == 1
+{
+    
+    //ghost var copyGraph: Graph := graph;
+    //assert isValidGraph(graph);
+    //If it belongs to the graph
+    if v in graph.0 then 
+        //assert isValidGraph(graph);
         //If there are edges incident of it 
         if (exists e: Edge | e in graph.1 :: v in e ) then
+            //assert isValidGraph(graph);
             //The vertex is "split" such that all those edges still exist but connect to different new nodes
             var edgesToChange: set<Edge> := incidentEdges(graph, v);
             var newNodes: set<Node> := addMultipleGreater(graph.0, |edgesToChange|); 
             assert(|newNodes| == |edgesToChange|);
+            incidentEdgesContainsNeighbors(graph, v, edgesToChange);
             var setNewEdges: set<Edge> := newSplitEdges(graph, newNodes, edgesToChange, v);
             ghost var g := (graph.0 - {v} + newNodes, graph.1 - edgesToChange + setNewEdges);
-            assert forall e | e in setNewEdges :: (|e| == 2 && exists a, b :: a in newNodes && b in graph.0 && a != b && e == {a, b});
-            assume{:axiom} false;
+
+            //Proof for isValidGraph(r)
+            //assert isValidGraph(graph);
+            assert forall e | e in setNewEdges :: |e| == 2;
+            assert forall e | e in setNewEdges :: (exists a, b :: a in newNodes && b in graph.0 && a != b && e == {a, b});
+            assert newNodes <= g.0;
+            removeVertexValid(graph, v);
+            assert isValidGraph((graph.0 - {v}, graph.1 - incidentEdges(graph, v)));
+            assert forall e | e in g.1 :: (|e| == 2 && exists u,v :: u in g.0 && v in g.0 && u != v && e == {u,v});
+
+            //Proof for forall n: Node | n in (r.0 - graph.0) :: |(set e: Edge | e in (r.1) && n in e :: e)| == 1
+            //assert isValidGraph(graph);
+            //assert (g.0 - graph.0) == newNodes;
+            //assert forall n: Node | n in newNodes :: n !in graph.0;
+            //assert isValidGraph(graph);
+            //notAVertexImpliesNotInAnEdgeSet(graph, newNodes);
+            //assert forall e: Edge, n: Node | e in graph.1 && n in newNodes :: n !in e;
+
             (graph.0 - {v} + newNodes, graph.1 - edgesToChange + setNewEdges)
         //If no edges are incident on it, the vertex is removed
         else (graph.0 - {v}, graph.1)
