Especificaciones/VertexCover/VertexCoverProperties.dfy
@@ -40,3 +40,13 @@ ensures !exists I:set<Node> | I <= graph.0 && |I| < k  :: isVertexCover(I,graph)
         assert false;
     }
 }
+
+lemma cardinalityVertexCoverLemma(g: Graph, A: set<Node>)
+    requires isValidGraph(g)
+    requires A <= g.0
+    requires isVertexCover(A, g)
+    requires exists B: set<Node> :: B <= g.0 && isVertexCover(B, g) && |B| < |A|
+    ensures exists C: set<Node> :: optimalVertexCover(g, C) && |C| < |A|
+{
+
+}
