Turing Reducciones/VertexCover/SplitVertexAux.dfy
@@ -1,0 +1,82 @@
+include "../../Especificaciones/VertexCover/VertexCoverOpt.dfy"
+include "../../Especificaciones/VertexCover/VertexCoverProperties.dfy"
+
+lemma CommonVertexCover1(g: Graph, g': Graph, v: Node, I: set<Node>)
+    requires isValidGraph(g)
+    requires isValidGraph(g')
+    requires splitVertex(g, v) == g'
+    requires I <= g.0
+    requires isVertexCover(I, g)
+    requires v in g.0
+    requires v !in I
+    ensures isVertexCover(I, g')
+{
+    assert v !in I;
+    assert neighborsOf(g, v) <= I;
+    assert neighborsOf(g, v) <= g'.0;
+    neighborsAreConnected(g, v, neighborsOf(g, v));
+    var difEdges: set<Edge> := g'.1 - g.1;
+    assert forall e: Edge | e in difEdges :: exists m: Node :: m in neighborsOf(g, v) && m in e;
+    assert forall e | e in difEdges :: |I * e| > 0;
+}
+
+lemma CommonOptimalVertexCover(g: Graph, g': Graph, v: Node, I: set<Node>)
+    requires isValidGraph(g)
+    requires isValidGraph(g')
+    requires splitVertex(g, v) == g'
+    requires I <= g.0
+    requires optimalVertexCover(g, I)
+    requires v in g.0
+    requires v !in I
+    ensures optimalVertexCover(g', I)
+{
+    
+    if !optimalVertexCover(g', I) {
+        CommonVertexCover1(g, g', v, I);
+        neighborsAreConnected(g, v, neighborsOf(g, v));
+        assert isVertexCover(I, g');
+        assert I <= g'.0;
+        assert !(forall S: set<Node> | S <= g'.0 && isVertexCover(S, g') :: |S| >= |I|) by {
+            if forall S: set<Node> | S <= g'.0 && isVertexCover(S, g') :: |S| >= |I|  {
+                assert forall S: set<Node> | S <= g'.0 && isVertexCover(S, g') :: |S| >= |I|;
+                assert isVertexCover(I, g');
+                assert I <= g'.0;
+                assert optimalVertexCover(g', I);
+                assert !optimalVertexCover(g', I);
+            }
+        }
+        assert exists S: set<Node> :: S <= g'.0 && isVertexCover(S, g') && |S| < |I|;
+        assume false;
+        var S: set<Node> :| optimalVertexCover(g', S) && |S| < |I|;
+        //var S: set<Node> :| optimalVertexCover(g', S) && |S| < |I|;
+        if neighborsOf(g, v) <= I {
+            assume false;
+            assert v !in I;
+            assert neighborsOf(g, v) <= I;
+            var difEdges: set<Edge> := g'.1 - g.1;
+            assert forall e: Edge | e in difEdges :: exists m: Node :: m in neighborsOf(g, v) && m in e;
+            assert optimalVertexCover(g, S);
+        }
+        assume{:axiom} false;
+    }
+}
+
+lemma splitHasGreaterOrEqualCover(g: Graph, g': Graph, v: Node, k: nat, k': nat)
+    requires isValidGraph(g)
+    requires isValidGraph(g')
+    requires splitVertex(g, v) == g'
+    requires optimalValueVertexCover(g, k)
+    requires optimalValueVertexCover(g', k')
+    ensures k' >= k
+{
+    //assert forall I: set<Node> | I <= g.0 && optimalVertexCover(g, I) :: v in I || v !in I;
+    if exists I: set<Node> | I <= g.0 && optimalVertexCover(g, I) :: v !in I {
+        assert exists I: set<Node> :: I <= g.0 && optimalVertexCover(g, I) && v !in I;
+        var I: set<Node> :| I <= g.0 && optimalVertexCover(g, I) && v !in I;
+        //assert isVertexCover(I, g');
+        assume false;
+    }
+    else{
+        assume false;
+    }
+}
